Smallstep.v
@@ -1,17 +1,23 @@
-(* from CompCert Smallstep.v *)
-
-Require Import Common.
+Require Import Relations.
+Require Import Wellfounded.
+Require Import Coqlib.
 Require Import Events.
 
 Set Implicit Arguments.
+
 Section CLOSURES.
 
 Variable genv: Type.
 Variable state: Type.
 Variable step: genv -> state -> trace -> state -> Prop.
 
+(** No transitions: stuck state *)
+
 Definition nostep (ge: genv) (s: state) : Prop :=
   forall t s', ~(step ge s t s').
+
+(** Zero, one or several transitions.  Also known as Kleene closure,
+    or reflexive transitive closure. *)
 
 Inductive star (ge: genv): state -> trace -> state -> Prop :=
   | star_refl: forall s,
@@ -20,62 +26,692 @@ Inductive star (ge: genv): state -> trace -> state -> Prop :=
       step ge s1 t1 s2 -> star ge s2 t2 s3 -> t = t1 ** t2 ->
       star ge s1 t s3.
 
+Lemma star_one:
+  forall ge s1 t s2, step ge s1 t s2 -> star ge s1 t s2.
+Proof.
+  intros. eapply star_step; eauto. apply star_refl. traceEq.
+Qed.
+
+Lemma star_trans:
+  forall ge s1 t1 s2, star ge s1 t1 s2 ->
+  forall t2 s3 t, star ge s2 t2 s3 -> t = t1 ** t2 -> star ge s1 t s3.
+Proof.
+  induction 1; intros.
+  rewrite H0. simpl. auto.
+  eapply star_step; eauto. traceEq.
+Qed.
+
+Lemma star_left:
+  forall ge s1 t1 s2 t2 s3 t,
+  step ge s1 t1 s2 -> star ge s2 t2 s3 -> t = t1 ** t2 ->
+  star ge s1 t s3.
+Proof star_step.
+
+Lemma star_right:
+  forall ge s1 t1 s2 t2 s3 t,
+  star ge s1 t1 s2 -> step ge s2 t2 s3 -> t = t1 ** t2 ->
+  star ge s1 t s3.
+Proof.
+  intros. eapply star_trans. eauto. apply star_one. eauto. auto.
+Qed.
+
+Lemma star_E0_ind:
+  forall ge (P: state -> state -> Prop),
+  (forall s, P s s) ->
+  (forall s1 s2 s3, step ge s1 E0 s2 -> P s2 s3 -> P s1 s3) ->
+  forall s1 s2, star ge s1 E0 s2 -> P s1 s2.
+Proof.
+  intros ge P BASE REC.
+  assert (forall s1 t s2, star ge s1 t s2 -> t = E0 -> P s1 s2).
+    induction 1; intros; subst.
+    auto.
+    destruct (Eapp_E0_inv _ _ H2). subst. eauto.
+  eauto.
+Qed.
+
+(** One or several transitions.  Also known as the transitive closure. *)
+
+Inductive plus (ge: genv): state -> trace -> state -> Prop :=
+  | plus_left: forall s1 t1 s2 t2 s3 t,
+      step ge s1 t1 s2 -> star ge s2 t2 s3 -> t = t1 ** t2 ->
+      plus ge s1 t s3.
+
+Lemma plus_one:
+  forall ge s1 t s2,
+  step ge s1 t s2 -> plus ge s1 t s2.
+Proof.
+  intros. econstructor; eauto. apply star_refl. traceEq.
+Qed.
+
+Lemma plus_star:
+  forall ge s1 t s2, plus ge s1 t s2 -> star ge s1 t s2.
+Proof.
+  intros. inversion H; subst.
+  eapply star_step; eauto.
+Qed.
+
+Lemma plus_right:
+  forall ge s1 t1 s2 t2 s3 t,
+  star ge s1 t1 s2 -> step ge s2 t2 s3 -> t = t1 ** t2 ->
+  plus ge s1 t s3.
+Proof.
+  intros. inversion H; subst. simpl. apply plus_one. auto.
+  rewrite Eapp_assoc. eapply plus_left; eauto.
+  eapply star_right; eauto.
+Qed.
+
+Lemma plus_left':
+  forall ge s1 t1 s2 t2 s3 t,
+  step ge s1 t1 s2 -> plus ge s2 t2 s3 -> t = t1 ** t2 ->
+  plus ge s1 t s3.
+Proof.
+  intros. eapply plus_left; eauto. apply plus_star; auto.
+Qed.
+
+Lemma plus_right':
+  forall ge s1 t1 s2 t2 s3 t,
+  plus ge s1 t1 s2 -> step ge s2 t2 s3 -> t = t1 ** t2 ->
+  plus ge s1 t s3.
+Proof.
+  intros. eapply plus_right; eauto. apply plus_star; auto.
+Qed.
+
+Lemma plus_star_trans:
+  forall ge s1 t1 s2 t2 s3 t,
+  plus ge s1 t1 s2 -> star ge s2 t2 s3 -> t = t1 ** t2 -> plus ge s1 t s3.
+Proof.
+  intros. inversion H; subst.
+  econstructor; eauto. eapply star_trans; eauto.
+  traceEq.
+Qed.
+
+Lemma star_plus_trans:
+  forall ge s1 t1 s2 t2 s3 t,
+  star ge s1 t1 s2 -> plus ge s2 t2 s3 -> t = t1 ** t2 -> plus ge s1 t s3.
+Proof.
+  intros. inversion H; subst.
+  simpl; auto.
+  rewrite Eapp_assoc.
+  econstructor. eauto. eapply star_trans. eauto.
+  apply plus_star. eauto. eauto. auto.
+Qed.
+
+Lemma plus_trans:
+  forall ge s1 t1 s2 t2 s3 t,
+  plus ge s1 t1 s2 -> plus ge s2 t2 s3 -> t = t1 ** t2 -> plus ge s1 t s3.
+Proof.
+  intros. eapply plus_star_trans. eauto. apply plus_star. eauto. auto.
+Qed.
+
+Lemma plus_inv:
+  forall ge s1 t s2,
+  plus ge s1 t s2 ->
+  step ge s1 t s2 \/ exists s', exists t1, exists t2, step ge s1 t1 s' /\ plus ge s' t2 s2 /\ t = t1 ** t2.
+Proof.
+  intros. inversion H; subst. inversion H1; subst.
+  left. rewrite E0_right. auto.
+  right. exists s3; exists t1; exists (t0 ** t3); split. auto.
+  split. econstructor; eauto. auto.
+Qed.
+
+Lemma star_inv:
+  forall ge s1 t s2,
+  star ge s1 t s2 ->
+  (s2 = s1 /\ t = E0) \/ plus ge s1 t s2.
+Proof.
+  intros. inv H. left; auto. right; econstructor; eauto.
+Qed.
+
+Lemma plus_ind2:
+  forall ge (P: state -> trace -> state -> Prop),
+  (forall s1 t s2, step ge s1 t s2 -> P s1 t s2) ->
+  (forall s1 t1 s2 t2 s3 t,
+   step ge s1 t1 s2 -> plus ge s2 t2 s3 -> P s2 t2 s3 -> t = t1 ** t2 ->
+   P s1 t s3) ->
+  forall s1 t s2, plus ge s1 t s2 -> P s1 t s2.
+Proof.
+  intros ge P BASE IND.
+  assert (forall s1 t s2, star ge s1 t s2 ->
+         forall s0 t0, step ge s0 t0 s1 ->
+         P s0 (t0 ** t) s2).
+  induction 1; intros.
+  rewrite E0_right. apply BASE; auto.
+  eapply IND. eauto. econstructor; eauto. subst t. eapply IHstar; eauto. auto.
+
+  intros. inv H0. eauto.
+Qed.
+
+Lemma plus_E0_ind:
+  forall ge (P: state -> state -> Prop),
+  (forall s1 s2 s3, step ge s1 E0 s2 -> star ge s2 E0 s3 -> P s1 s3) ->
+  forall s1 s2, plus ge s1 E0 s2 -> P s1 s2.
+Proof.
+  intros. inv H0. exploit Eapp_E0_inv; eauto. intros [A B]; subst. eauto.
+Qed.
+
+(** Counted sequences of transitions *)
+
+Inductive starN (ge: genv): nat -> state -> trace -> state -> Prop :=
+  | starN_refl: forall s,
+      starN ge O s E0 s
+  | starN_step: forall n s t t1 s' t2 s'',
+      step ge s t1 s' -> starN ge n s' t2 s'' -> t = t1 ** t2 ->
+      starN ge (S n) s t s''.
+
+Remark starN_star:
+  forall ge n s t s', starN ge n s t s' -> star ge s t s'.
+Proof.
+  induction 1; econstructor; eauto.
+Qed.
+
+Remark star_starN:
+  forall ge s t s', star ge s t s' -> exists n, starN ge n s t s'.
+Proof.
+  induction 1.
+  exists O; constructor.
+  destruct IHstar as [n P]. exists (S n); econstructor; eauto.
+Qed.
+
+(** Infinitely many transitions *)
+
 CoInductive forever (ge: genv): state -> traceinf -> Prop :=
   | forever_intro: forall s1 t s2 T,
       step ge s1 t s2 -> forever ge s2 T ->
       forever ge s1 (t *** T).
+
+Lemma star_forever:
+  forall ge s1 t s2, star ge s1 t s2 ->
+  forall T, forever ge s2 T ->
+  forever ge s1 (t *** T).
+Proof.
+  induction 1; intros. simpl. auto.
+  subst t. rewrite Eappinf_assoc.
+  econstructor; eauto.
+Qed.
+
+(** An alternate, equivalent definition of [forever] that is useful
+    for coinductive reasoning. *)
+
+Variable A: Type.
+Variable order: A -> A -> Prop.
+
+CoInductive forever_N (ge: genv) : A -> state -> traceinf -> Prop :=
+  | forever_N_star: forall s1 t s2 a1 a2 T1 T2,
+      star ge s1 t s2 ->
+      order a2 a1 ->
+      forever_N ge a2 s2 T2 ->
+      T1 = t *** T2 ->
+      forever_N ge a1 s1 T1
+  | forever_N_plus: forall s1 t s2 a1 a2 T1 T2,
+      plus ge s1 t s2 ->
+      forever_N ge a2 s2 T2 ->
+      T1 = t *** T2 ->
+      forever_N ge a1 s1 T1.
+
+Hypothesis order_wf: well_founded order.
+
+Lemma forever_N_inv:
+  forall ge a s T,
+  forever_N ge a s T ->
+  exists t, exists s', exists a', exists T',
+  step ge s t s' /\ forever_N ge a' s' T' /\ T = t *** T'.
+Proof.
+  intros ge a0. pattern a0. apply (well_founded_ind order_wf).
+  intros. inv H0.
+  (* star case *)
+  inv H1.
+  (* no transition *)
+  change (E0 *** T2) with T2. apply H with a2. auto. auto.
+  (* at least one transition *)
+  exists t1; exists s0; exists x; exists (t2 *** T2).
+  split. auto. split. eapply forever_N_star; eauto.
+  apply Eappinf_assoc.
+  (* plus case *)
+  inv H1.
+  exists t1; exists s0; exists a2; exists (t2 *** T2).
+  split. auto.
+  split. inv H3. auto.
+  eapply forever_N_plus. econstructor; eauto. eauto. auto.
+  apply Eappinf_assoc.
+Qed.
+
+Lemma forever_N_forever:
+  forall ge a s T, forever_N ge a s T -> forever ge s T.
+Proof.
+  cofix COINDHYP; intros.
+  destruct (forever_N_inv H) as [t [s' [a' [T' [P [Q R]]]]]].
+  rewrite R. apply forever_intro with s'. auto.
+  apply COINDHYP with a'; auto.
+Qed.
+
+(** Yet another alternative definition of [forever]. *)
+
+CoInductive forever_plus (ge: genv) : state -> traceinf -> Prop :=
+  | forever_plus_intro: forall s1 t s2 T1 T2,
+      plus ge s1 t s2 ->
+      forever_plus ge s2 T2 ->
+      T1 = t *** T2 ->
+      forever_plus ge s1 T1.
+
+Lemma forever_plus_inv:
+  forall ge s T,
+  forever_plus ge s T ->
+  exists s', exists t, exists T',
+  step ge s t s' /\ forever_plus ge s' T' /\ T = t *** T'.
+Proof.
+  intros. inv H. inv H0. exists s0; exists t1; exists (t2 *** T2).
+  split. auto.
+  split. exploit star_inv; eauto. intros [[P Q] | R].
+    subst. simpl. auto. econstructor; eauto.
+  traceEq.
+Qed.
+
+Lemma forever_plus_forever:
+  forall ge s T, forever_plus ge s T -> forever ge s T.
+Proof.
+  cofix COINDHYP; intros.
+  destruct (forever_plus_inv H) as [s' [t [T' [P [Q R]]]]].
+  subst. econstructor; eauto.
+Qed.
+
+(** Infinitely many silent transitions *)
 
 CoInductive forever_silent (ge: genv): state -> Prop :=
   | forever_silent_intro: forall s1 s2,
       step ge s1 E0 s2 -> forever_silent ge s2 ->
       forever_silent ge s1.
 
+(** An alternate definition. *)
+
+CoInductive forever_silent_N (ge: genv) : A -> state -> Prop :=
+  | forever_silent_N_star: forall s1 s2 a1 a2,
+      star ge s1 E0 s2 ->
+      order a2 a1 ->
+      forever_silent_N ge a2 s2 ->
+      forever_silent_N ge a1 s1
+  | forever_silent_N_plus: forall s1 s2 a1 a2,
+      plus ge s1 E0 s2 ->
+      forever_silent_N ge a2 s2 ->
+      forever_silent_N ge a1 s1.
+
+Lemma forever_silent_N_inv:
+  forall ge a s,
+  forever_silent_N ge a s ->
+  exists s', exists a',
+  step ge s E0 s' /\ forever_silent_N ge a' s'.
+Proof.
+  intros ge a0. pattern a0. apply (well_founded_ind order_wf).
+  intros. inv H0.
+  (* star case *)
+  inv H1.
+  (* no transition *)
+  apply H with a2. auto. auto.
+  (* at least one transition *)
+  exploit Eapp_E0_inv; eauto. intros [P Q]. subst.
+  exists s0; exists x.
+  split. auto. eapply forever_silent_N_star; eauto.
+  (* plus case *)
+  inv H1. exploit Eapp_E0_inv; eauto. intros [P Q]. subst.
+  exists s0; exists a2.
+  split. auto. inv H3. auto.
+  eapply forever_silent_N_plus. econstructor; eauto. eauto.
+Qed.
+
+Lemma forever_silent_N_forever:
+  forall ge a s, forever_silent_N ge a s -> forever_silent ge s.
+Proof.
+  cofix COINDHYP; intros.
+  destruct (forever_silent_N_inv H) as [s' [a' [P Q]]].
+  apply forever_silent_intro with s'. auto.
+  apply COINDHYP with a'; auto.
+Qed.
+
+(** Infinitely many non-silent transitions *)
+
 CoInductive forever_reactive (ge: genv): state -> traceinf -> Prop :=
   | forever_reactive_intro: forall s1 s2 t T,
       star ge s1 t s2 -> t <> E0 -> forever_reactive ge s2 T ->
       forever_reactive ge s1 (t *** T).
 
+Lemma star_forever_reactive:
+  forall ge s1 t s2 T,
+  star ge s1 t s2 -> forever_reactive ge s2 T ->
+  forever_reactive ge s1 (t *** T).
+Proof.
+  intros. inv H0. rewrite <- Eappinf_assoc. econstructor.
+  eapply star_trans; eauto.
+  red; intro. exploit Eapp_E0_inv; eauto. intros [P Q]. contradiction.
+  auto.
+Qed.
+
 End CLOSURES.
+
+(** * Transition semantics *)
+
+(** The general form of a transition semantics. *)
 
 Record semantics : Type := Semantics_gen {
   state: Type;
   genvtype: Type;
   step : genvtype -> state -> trace -> state -> Prop;
   initial_state: state -> Prop;
-  final_state: state -> Prop;   (* we don't have a return value *)
+  final_state: state -> Prop;
   globalenv: genvtype;
 }.
 
 Notation " 'Step' L " := (step L (globalenv L)) (at level 1) : smallstep_scope.
 Notation " 'Star' L " := (star (step L) (globalenv L)) (at level 1) : smallstep_scope.
+Notation " 'Plus' L " := (plus (step L) (globalenv L)) (at level 1) : smallstep_scope.
 Notation " 'Forever_silent' L " := (forever_silent (step L) (globalenv L)) (at level 1) : smallstep_scope.
 Notation " 'Forever_reactive' L " := (forever_reactive (step L) (globalenv L)) (at level 1) : smallstep_scope.
 Notation " 'Nostep' L " := (nostep (step L) (globalenv L)) (at level 1) : smallstep_scope.
+
 Open Scope smallstep_scope.
 
+(** * Forward simulations between two transition semantics. *)
 
-(* removed return value and order (measure) *)
-Record fsim_properties (L1 L2: semantics)
-       (match_states: state L1 -> state L2 -> Prop) : Prop := {
+(** The general form of a forward simulation. *)
+
+Record fsim_properties (L1 L2: semantics) (index: Type)
+                       (order: index -> index -> Prop)
+                       (match_states: index -> state L1 -> state L2 -> Prop) : Prop := {
+    fsim_order_wf: well_founded order;
     fsim_match_initial_states:
       forall s1, initial_state L1 s1 ->
-      exists s2, initial_state L2 s2 /\ match_states s1 s2;
+      exists i, exists s2, initial_state L2 s2 /\ match_states i s1 s2;
     fsim_match_final_states:
-      forall s1 s2,
-      match_states s1 s2 -> final_state L1 s1 -> final_state L2 s2;
+      forall i s1 s2,
+      match_states i s1 s2 -> final_state L1 s1 -> final_state L2 s2;
     fsim_simulation:
       forall s1 t s1', Step L1 s1 t s1' ->
-      forall s2, match_states s1 s2 ->
-      exists s2',
-         (Step L2 s2 t s2') /\ match_states s1' s2';
+      forall i s2, match_states i s1 s2 ->
+      exists i', exists s2',
+         (Plus L2 s2 t s2' \/ (Star L2 s2 t s2' /\ order i' i))
+      /\ match_states i' s1' s2';
   }.
 
 Arguments fsim_properties: clear implicits.
 
 Inductive forward_simulation (L1 L2: semantics) : Prop :=
-  Forward_simulation (match_states: state L1 -> state L2 -> Prop)
-                     (props: fsim_properties L1 L2 match_states).
+  Forward_simulation (index: Type)
+                     (order: index -> index -> Prop)
+                     (match_states: index -> state L1 -> state L2 -> Prop)
+                     (props: fsim_properties L1 L2 index order match_states).
 
-Arguments Forward_simulation {L1 L2} match_states props.
+Arguments Forward_simulation {L1 L2 index} order match_states props.
 
+(** An alternate form of the simulation diagram *)
 
+Lemma fsim_simulation':
+  forall L1 L2 index order match_states, fsim_properties L1 L2 index order match_states ->
+  forall i s1 t s1', Step L1 s1 t s1' ->
+  forall s2, match_states i s1 s2 ->
+  (exists i', exists s2', Plus L2 s2 t s2' /\ match_states i' s1' s2')
+  \/ (exists i', order i' i /\ t = E0 /\ match_states i' s1' s2).
+Proof.
+  intros. exploit fsim_simulation; eauto.
+  intros [i' [s2' [A B]]]. intuition.
+  left; exists i'; exists s2'; auto.
+  inv H3.
+  right; exists i'; auto.
+  left; exists i'; exists s2'; split; auto. econstructor; eauto.
+Qed.
+
+(** ** Forward simulation diagrams. *)
+
+(** Various simulation diagrams that imply forward simulation *)
+
+Section FORWARD_SIMU_DIAGRAMS.
+
+Variable L1: semantics.
+Variable L2: semantics.
+
+Variable match_states: state L1 -> state L2 -> Prop.
+
+Hypothesis match_initial_states:
+  forall s1, initial_state L1 s1 ->
+  exists s2, initial_state L2 s2 /\ match_states s1 s2.
+
+Hypothesis match_final_states:
+  forall s1 s2,
+  match_states s1 s2 ->
+  final_state L1 s1 ->
+  final_state L2 s2.
+
+(** Simulation when one transition in the first program
+    corresponds to zero, one or several transitions in the second program.
+    However, there is no stuttering: infinitely many transitions
+    in the source program must correspond to infinitely many
+    transitions in the second program. *)
+
+Section SIMULATION_STAR_WF.
+
+(** [order] is a well-founded ordering associated with states
+  of the first semantics.  Stuttering steps must correspond
+  to states that decrease w.r.t. [order]. *)
+
+Variable order: state L1 -> state L1 -> Prop.
+Hypothesis order_wf: well_founded order.
+
+Hypothesis simulation:
+  forall s1 t s1', Step L1 s1 t s1' ->
+  forall s2, match_states s1 s2 ->
+  exists s2',
+  (Plus L2 s2 t s2' \/ (Star L2 s2 t s2' /\ order s1' s1))
+  /\ match_states s1' s2'.
+
+Lemma forward_simulation_star_wf: forward_simulation L1 L2.
+Proof.
+  apply Forward_simulation with order (fun idx s1 s2 => idx = s1 /\ match_states s1 s2);
+  constructor.
+- auto.
+- intros. exploit match_initial_states; eauto. intros [s2 [A B]].
+    exists s1; exists s2; auto.
+- intros. destruct H. eapply match_final_states; eauto.
+- intros. destruct H0. subst i. exploit simulation; eauto. intros [s2' [A B]].
+  exists s1'; exists s2'; intuition auto.
+Qed.
+
+End SIMULATION_STAR_WF.
+
+Section SIMULATION_STAR.
+
+(** We now consider the case where we have a nonnegative integer measure
+  associated with states of the first semantics.  It must decrease when we take
+  a stuttering step. *)
+
+Variable measure: state L1 -> nat.
+
+Hypothesis simulation:
+  forall s1 t s1', Step L1 s1 t s1' ->
+  forall s2, match_states s1 s2 ->
+  (exists s2', Plus L2 s2 t s2' /\ match_states s1' s2')
+  \/ (measure s1' < measure s1 /\ t = E0 /\ match_states s1' s2)%nat.
+
+Lemma forward_simulation_star: forward_simulation L1 L2.
+Proof.
+  apply forward_simulation_star_wf with (ltof _ measure).
+  apply well_founded_ltof.
+  intros. exploit simulation; eauto. intros [[s2' [A B]] | [A [B C]]].
+  exists s2'; auto.
+  exists s2; split. right; split. rewrite B. apply star_refl. auto. auto.
+Qed.
+
+End SIMULATION_STAR.
+
+(** Simulation when one transition in the first program corresponds
+    to one or several transitions in the second program. *)
+
+Section SIMULATION_PLUS.
+
+Hypothesis simulation:
+  forall s1 t s1', Step L1 s1 t s1' ->
+  forall s2, match_states s1 s2 ->
+  exists s2', Plus L2 s2 t s2' /\ match_states s1' s2'.
+
+Lemma forward_simulation_plus: forward_simulation L1 L2.
+Proof.
+  apply forward_simulation_star with (measure := fun _ => O).
+  intros. exploit simulation; eauto.
+Qed.
+
+End SIMULATION_PLUS.
+
+(** Lock-step simulation: each transition in the first semantics
+    corresponds to exactly one transition in the second semantics. *)
+
+Section SIMULATION_STEP.
+
+Hypothesis simulation:
+  forall s1 t s1', Step L1 s1 t s1' ->
+  forall s2, match_states s1 s2 ->
+  exists s2', Step L2 s2 t s2' /\ match_states s1' s2'.
+
+Lemma forward_simulation_step: forward_simulation L1 L2.
+Proof.
+  apply forward_simulation_plus.
+  intros. exploit simulation; eauto. intros [s2' [A B]].
+  exists s2'; split; auto. apply plus_one; auto.
+Qed.
+
+End SIMULATION_STEP.
+
+(** Simulation when one transition in the first program
+    corresponds to zero or one transitions in the second program.
+    However, there is no stuttering: infinitely many transitions
+    in the source program must correspond to infinitely many
+    transitions in the second program. *)
+
+Section SIMULATION_OPT.
+
+Variable measure: state L1 -> nat.
+
+Hypothesis simulation:
+  forall s1 t s1', Step L1 s1 t s1' ->
+  forall s2, match_states s1 s2 ->
+  (exists s2', Step L2 s2 t s2' /\ match_states s1' s2')
+  \/ (measure s1' < measure s1 /\ t = E0 /\ match_states s1' s2)%nat.
+
+Lemma forward_simulation_opt: forward_simulation L1 L2.
+Proof.
+  apply forward_simulation_star with measure.
+  intros. exploit simulation; eauto. intros [[s2' [A B]] | [A [B C]]].
+  left; exists s2'; split; auto. apply plus_one; auto.
+  right; auto.
+Qed.
+
+End SIMULATION_OPT.
+
+End FORWARD_SIMU_DIAGRAMS.
+
+(** ** Forward simulation of transition sequences *)
+
+Section SIMULATION_SEQUENCES.
+
+Context L1 L2 index order match_states (S: fsim_properties L1 L2 index order match_states).
+
+Lemma simulation_star:
+  forall s1 t s1', Star L1 s1 t s1' ->
+  forall i s2, match_states i s1 s2 ->
+  exists i', exists s2', Star L2 s2 t s2' /\ match_states i' s1' s2'.
+Proof.
+  induction 1; intros.
+  exists i; exists s2; split; auto. apply star_refl.
+  exploit fsim_simulation; eauto. intros [i' [s2' [A B]]].
+  exploit IHstar; eauto. intros [i'' [s2'' [C D]]].
+  exists i''; exists s2''; split; auto. eapply star_trans; eauto.
+  intuition auto. apply plus_star; auto.
+Qed.
+
+Lemma simulation_plus:
+  forall s1 t s1', Plus L1 s1 t s1' ->
+  forall i s2, match_states i s1 s2 ->
+  (exists i', exists s2', Plus L2 s2 t s2' /\ match_states i' s1' s2')
+  \/ (exists i', clos_trans _ order i' i /\ t = E0 /\ match_states i' s1' s2).
+Proof.
+  induction 1 using plus_ind2; intros.
+(* base case *)
+  exploit fsim_simulation'; eauto. intros [A | [i' A]].
+  left; auto.
+  right; exists i'; intuition.
+(* inductive case *)
+  exploit fsim_simulation'; eauto. intros [[i' [s2' [A B]]] | [i' [A [B C]]]].
+  exploit simulation_star. apply plus_star; eauto. eauto.
+  intros [i'' [s2'' [P Q]]].
+  left; exists i''; exists s2''; split; auto. eapply plus_star_trans; eauto.
+  exploit IHplus; eauto. intros [[i'' [s2'' [P Q]]] | [i'' [P [Q R]]]].
+  subst. simpl. left; exists i''; exists s2''; auto.
+  subst. simpl. right; exists i''; intuition auto.
+  eapply t_trans; eauto. eapply t_step; eauto.
+Qed.
+
+Lemma simulation_forever_silent:
+  forall i s1 s2,
+  Forever_silent L1 s1 -> match_states i s1 s2 ->
+  Forever_silent L2 s2.
+Proof.
+  assert (forall i s1 s2,
+          Forever_silent L1 s1 -> match_states i s1 s2 ->
+          forever_silent_N (step L2) order (globalenv L2) i s2).
+    cofix COINDHYP; intros.
+    inv H. destruct (fsim_simulation S _ _ _ H1 _ _ H0) as [i' [s2' [A B]]].
+    destruct A as [C | [C D]].
+    eapply forever_silent_N_plus; eauto.
+    eapply forever_silent_N_star; eauto.
+  intros. eapply forever_silent_N_forever; eauto. eapply fsim_order_wf; eauto.
+Qed.
+
+Lemma simulation_forever_reactive:
+  forall i s1 s2 T,
+  Forever_reactive L1 s1 T -> match_states i s1 s2 ->
+  Forever_reactive L2 s2 T.
+Proof.
+  cofix COINDHYP; intros.
+  inv H.
+  edestruct simulation_star as [i' [st2' [A B]]]; eauto.
+  econstructor; eauto.
+Qed.
+
+End SIMULATION_SEQUENCES.
+
+(** ** Composing two forward simulations *)
+
+Lemma compose_forward_simulations:
+  forall L1 L2 L3, forward_simulation L1 L2 -> forward_simulation L2 L3 -> forward_simulation L1 L3.
+Proof.
+  intros L1 L2 L3 S12 S23. 
+  destruct S12 as [index order match_states props].
+  destruct S23 as [index' order' match_states' props'].
+
+  set (ff_index := (index' * index)%type).
+  set (ff_order := lex_ord (clos_trans _ order') order).
+  set (ff_match_states := fun (i: ff_index) (s1: state L1) (s3: state L3) =>
+                             exists s2, match_states (snd i) s1 s2 /\ match_states' (fst i) s2 s3).
+  apply Forward_simulation with ff_order ff_match_states; constructor.
+- (* well founded *)
+  unfold ff_order. apply wf_lex_ord. apply wf_clos_trans.
+  eapply fsim_order_wf; eauto. eapply fsim_order_wf; eauto.
+- (* initial states *)
+  intros. exploit (fsim_match_initial_states props); eauto. intros [i [s2 [A B]]].
+  exploit (fsim_match_initial_states props'); eauto. intros [i' [s3 [C D]]].
+  exists (i', i); exists s3; split; auto. exists s2; auto.
+- (* final states *)
+  intros. destruct H as [s3 [A B]].
+  eapply (fsim_match_final_states props'); eauto.
+  eapply (fsim_match_final_states props); eauto.
+- (* simulation *)
+  intros. destruct H0 as [s3 [A B]]. destruct i as [i2 i1]; simpl in *.
+  exploit (fsim_simulation' props); eauto. intros [[i1' [s3' [C D]]] | [i1' [C [D E]]]].
++ (* L2 makes one or several steps. *)
+  exploit simulation_plus; eauto. intros [[i2' [s2' [P Q]]] | [i2' [P [Q R]]]].
+* (* L3 makes one or several steps *)
+  exists (i2', i1'); exists s2'; split. auto. exists s3'; auto.
+* (* L3 makes no step *)
+  exists (i2', i1'); exists s2; split.
+  right; split. subst t; apply star_refl. red. left. auto.
+  exists s3'; auto.
++ (* L2 makes no step *)
+  exists (i2, i1'); exists s2; split.
+  right; split. subst t; apply star_refl. red. right. auto.
+  exists s3; auto.
+Qed.
