LTT_PLTT.v
@@ -4,32 +4,11 @@ Require Import Machine.
 Require Import LTT.
 Require Import PLTT.
 Require Import Smallstep.
+Require Import Behavior.
 
 Module LTT_TO_PLTT.
 
 Include AbstractMachine.
-
-Inductive match_states (split : list Component.id)
-  : LTT.state -> PLTT.partial_state -> Prop :=
-| program_control:
-    forall C s ps mem pmem regs pc,
-      PLTT.is_program_component C split ->
-      ps = PLTT.to_partial_stack s split ->
-      PLTT.maps_match_on split mem pmem ->
-      match_states split
-                   (C, s, mem, regs, pc)
-                   (PLTT.PC (C, ps, pmem, regs, pc))
-
-| context_control:
-    forall C s ps mem pmem regs pc,
-      PLTT.is_context_component C split ->
-      ps = PLTT.to_partial_stack s split ->
-      PLTT.maps_match_on split mem pmem ->
-      match_states split
-                   (C, s, mem, regs, pc)
-                   (PLTT.CC (C, ps, pmem)).
-
-Hint Constructors match_states.
 
 Section SIMULATION.
   Variable p : LTT.program.
@@ -55,6 +34,39 @@ Section SIMULATION.
                              (LTT.prog_entrypoints p)
                              split.
 
+  Inductive match_states (split : list Component.id)
+    : LTT.state -> PLTT.partial_state -> Prop :=
+  | program_control:
+      forall C s ps mem pmem regs pc,
+        PLTT.is_program_component C split ->
+        ps = PLTT.to_partial_stack s split ->
+        PLTT.maps_match_on split mem pmem ->
+        match_states split
+                     (C, s, mem, regs, pc)
+                     (PLTT.PC (C, ps, pmem, regs, pc))
+
+  | context_control:
+      forall C s ps mem pmem regs pc,
+        PLTT.is_context_component C split ->
+        ps = PLTT.to_partial_stack s split ->
+        PLTT.maps_match_on split mem pmem ->
+        match_states split
+                     (C, s, mem, regs, pc)
+                     (PLTT.CC (C, ps, pmem) PLTT.Normal)
+
+  | context_went_wrong:
+      forall C s ps mem pmem regs pc,
+        PLTT.is_context_component C split ->
+        ps = PLTT.to_partial_stack s split ->
+        PLTT.maps_match_on split mem pmem ->
+        (forall s' t, ~ LTT.step G (C,s,mem,regs,pc) t s') ->
+        ~ LTT.final_state (C,s,mem,regs,pc) ->
+        match_states split
+                     (C, s, mem, regs, pc)
+                     (PLTT.CC (C, ps, pmem) PLTT.WentWrong).
+
+  Hint Constructors match_states.
+
   Lemma initial_states_match:
     forall s,
       LTT.initial_state p s ->
@@ -77,7 +89,7 @@ Section SIMULATION.
         apply program_control; try auto.
         * unfold PLTT.is_program_component.
           apply Util.in_iff_mem_true. auto.
-    - exists (PLTT.CC (0, [], mem)).
+    - exists (PLTT.CC (0, [], mem) PLTT.Normal).
       split.
       + unfold PLTT.initial_state.
         split; auto.
@@ -96,10 +108,10 @@ Section SIMULATION.
     intros s ps Hmatch_states Hs_final.
     destruct s
       as [[[[C d] mem] regs] pc] eqn:Hstate_s.
-    destruct Hs_final
-      as [empty_stack executing_halt].
-    unfold PLTT.final_state.
-    inversion Hmatch_states; subst; auto.
+    unfold LTT.final_state in Hs_final.
+    inversion Hmatch_states; subst;
+      unfold PLTT.final_state; auto.
+    - exfalso. apply H9. auto.
   Qed.
 
   Lemma lockstep_simulation:
@@ -131,7 +143,10 @@ Section SIMULATION.
     (* case analysis on who has control and on the execution *)
     inversion Hmatch_states as
         [ C d pd mem pmem regs pc Hcontrol Hpstack Hmem
-        | C d pd mem pmem regs pc Hcontrol Hpstack Hmem ]; subst;
+        | C d pd mem pmem regs pc Hcontrol Hpstack Hmem
+        | C d pd mem pmem regs pc Hcontrol Hpstack Hmem
+            Hno_step Hnot_final];
+      subst;
       inversion Hstep; subst;
 
         (* try to extract the current component interface *)
@@ -157,7 +172,10 @@ Section SIMULATION.
                | apply HCmem
                ]
              | auto
-            ]).
+            ]);
+
+        (* the context goes wrong *)
+        try (exfalso; eapply Hno_step; eauto).
 
     (* program store *)
     - exists (PLTT.PC (C, PLTT.to_partial_stack d split,
@@ -318,12 +336,125 @@ Section SIMULATION.
   Theorem forward_simulation_between_LTT_and_PLTT:
     forward_simulation (LTT.semantics p) (PLTT.semantics pp).
   Proof.
-    apply Forward_simulation with (match_states split).
-    constructor.
+    apply forward_simulation_step with (match_states split).
     - apply initial_states_match.
     - apply final_states_match.
     - rewrite p_transfto_pp.
       apply lockstep_simulation.
   Qed.
+
+  Corollary not_wrong_behavior_preservation:
+    forall beh,
+      not_wrong beh ->
+      program_behaves (LTT.semantics p) beh ->
+      program_behaves (PLTT.semantics pp) beh.
+  Proof.
+    intros beh Hnotwrong Hprogbeh.
+    eapply forward_simulation_same_safe_behavior; eauto.
+    apply forward_simulation_between_LTT_and_PLTT.
+  Qed.
+
+  Theorem wrong_behavior_preservation:
+    forall t,
+      program_behaves (LTT.semantics p) (Goes_wrong t) ->
+      program_behaves (PLTT.semantics pp) (Goes_wrong t).
+  Proof.
+    intros t Hprogbeh.
+    destruct forward_simulation_between_LTT_and_PLTT
+      as [index order generic_match_states S].
+    remember S as sim_prop.
+    destruct S as [? Hmatch_initial Hmatch_final Hsim].
+    inversion Hprogbeh.
+    - destruct (Hmatch_initial s) as [i]; auto.
+      destruct H2 as [ps [Hps_init Hps_match]].
+      apply program_runs with ps.
+      + auto.
+      + inversion H0.
+        destruct (simulation_star sim_prop H3 i ps Hps_match)
+          as [i' [ps' [Hps_star Hps'_match]]].
+        apply state_goes_wrong with ps'; auto.
+    (* stuck! I can't reason on our specific instance 
+       of match_states, hence I cannot demonstrate that 
+       PLTT cannot step! *)
+  Admitted.
+
+  Require Import Coqlib.
+  
+  Lemma nostep_aux:
+    forall s ps,
+      match_states split s ps ->
+      (forall s' t, ~ (LTT.step G s t s')) ->
+      (forall ps' t, ~ (PLTT.step G' ps t ps')).
+  Proof.
+    intros s ps Hmatch_states Hnostep.
+    destruct s
+      as [[[[C d] mem] regs] pc] eqn:Hstate_s.
+    inversion Hmatch_states; subst; intros.
+    - admit. (* feasible *)
+    - admit.
+    - intro contra. inversion contra.
+  Qed.
+
+  Section FORWARD_SIMULATION.
+    Context index order match_states
+            (S: fsim_properties (LTT.semantics p) (PLTT.semantics pp)
+                                index order match_states).
+
+    Lemma forward_simulation_state_behaves:
+      forall i s1 s2 beh,
+        match_states i s1 s2 ->
+        state_behaves (LTT.semantics p) s1 beh ->
+        state_behaves (PLTT.semantics pp) s2 beh.
+    Proof.
+      intros. inv H0.
+      - (* termination *)
+        exploit simulation_star; eauto. intros [i' [s2' [A B]]].
+        econstructor; eauto. eapply fsim_match_final_states; eauto.
+      - (* silent divergence *)
+        exploit simulation_star; eauto. intros [i' [s2' [A B]]].
+        econstructor; eauto. eapply simulation_forever_silent; eauto.
+      - (* reactive divergence *)
+        econstructor. eapply simulation_forever_reactive; eauto.
+      - (* going wrong *)
+        exploit simulation_star; eauto. intros [i' [s2' [A B]]].
+        econstructor; eauto.
+        (* stuck!! *)
+    Admitted.
+  End FORWARD_SIMULATION.
+
+  Theorem behavior_preservation':
+    forall beh,
+      program_behaves (LTT.semantics p) beh ->
+      program_behaves (PLTT.semantics pp) beh.
+  Proof.
+    intros beh Hprogbeh.
+    destruct (forward_simulation_behavior_improves
+                forward_simulation_between_LTT_and_PLTT
+                Hprogbeh) as [beh2 [Hprogbeh2 Hbehimp]].
+    destruct forward_simulation_between_LTT_and_PLTT
+      as [? ? generic_match_states S].
+    unfold behavior_improves in Hbehimp.
+    inversion Hbehimp.
+    - subst. auto.
+    - destruct H as [t [Hgoeswrong Hbehprefix]].
+      rewrite Hgoeswrong.
+      destruct Hprogbeh.
+      (* initial states *)
+      destruct (initial_states_match s H)
+          as [ps [Hps_init Hmatch_states]].
+      (* star simulation *)
+      inversion H0.
+      + subst. inversion H3.
+      + subst. inversion H3.
+      + subst. inversion H2.
+      + subst. inversion H4.
+        eapply program_runs.
+        * eauto.
+        * admit. (*eapply state_goes_wrong.
+          ** pose (simulation_star S H1).*)
+      + subst. inversion Hgoeswrong. subst.
+        apply program_goes_initially_wrong.
+        intros. unfold not. intro.
+  Admitted.
 End SIMULATION.
 End LTT_TO_PLTT.
